Extract instrumentation to a different file

io/ILang.CompileTo.MLang.fst
@@ -6,14 +6,16 @@ open FStar.Tactics.Typeclasses
 
 open Common
 
-open ILang
-open MLang
-open Hist
+open TC.Checkable
 open TC.Monitorable.Hist
 
 open IO.Sig
 open IIO
-open TC.Checkable
+
+open ILang
+open MLang
+
+open MLang.InstrumentTo.ILang
 
 class compilable (comp_in:Type) (pi:monitorable_prop) = {
   comp_out : Type;
@@ -121,176 +123,6 @@ instance backtranslateable_resexn pi (t:Type) {| d1:backtranslateable t pi |} : 
 }
 
 (** *** Instrumentable arrows **)
-let super_lemma 
-  (pi:monitorable_prop)
-  (m : iio (Universe.raise_t 'b))
-  d
-  k
-  p
-  (h:trace)
-  (_:squash (dm_iio_theta (Decorated d m k) p h))
-  (_:squash (forall h lt. d h lt ==> enforced_locally pi h lt)) :
-  Lemma (
-   dm_iio_theta m (fun lt r -> enforced_locally pi h lt) h /\
-   dm_iio_theta m
-      (fun lt r ->
-        dm_iio_theta (k (Universe.downgrade_val r))
-          (hist_post_shift p lt)
-          (apply_changes h lt)) h) = 
-  
-  calc (==>) {
-      dm_iio_theta (Decorated d m k) p h;
-      ==> { _ by (
-            binder_retype (nth_binder (-1));
-            norm [delta_only [`%dm_iio_theta;`%DMFree.theta]; zeta];
-            trefl ();
-            norm [delta_only [`%dm_iio_theta]];
-            assumption ()) }
-      hist_bind
-             (fun p h -> dm_iio_theta m (fun lt r -> d h lt /\ p lt r) h)
-             (fun r -> dm_iio_theta (k (Universe.downgrade_val r))) p h;
-      ==> {}
-      hist_bind
-             (fun p h -> dm_iio_theta m (fun lt r -> enforced_locally pi h lt /\ p lt r) h)
-             (fun r -> dm_iio_theta (k (Universe.downgrade_val r))) p h;
-      ==> { _ by (binder_retype (nth_binder (-1));
-                  norm [delta_only [`%hist_bind;`%hist_post_bind]]; trefl (); assumption ()) }
-      dm_iio_theta m
-        (fun lt r ->
-          enforced_locally pi h lt /\
-          dm_iio_theta (k (Universe.downgrade_val r))
-            (hist_post_shift p lt)
-            (List.Tot.Base.rev lt @ h)) h;
-      ==> {}
-      dm_iio_theta m
-        (fun lt r ->
-          dm_iio_theta (k (Universe.downgrade_val r))
-            (hist_post_shift p lt)
-            (List.Tot.Base.rev lt @ h)) h;
-    }
-
-
-let lemma_smt_pat (pi:monitorable_prop) (h lt1 lt2:trace) :
-  Lemma (requires (
-    enforced_locally pi h lt1 /\
-    enforced_locally pi (apply_changes h lt1) lt2))
-    (ensures (
-    enforced_locally pi h (lt1 @ lt2))) [SMTPat (enforced_locally pi h (lt1@lt2))] = (** not urgent **) admit ()
-
-let rec inside_respects_pi
-  (tree : iio (resexn 'a))
-  (pi : monitorable_prop) : Type0 =
-  match tree with
-  | Return _ -> True
-  | PartialCall pre k ->
-      pre ==> (inside_respects_pi (k ()) pi)
-  | Call cmd arg k ->
-      forall res. inside_respects_pi (k res) pi
-  | Decorated dec m k ->
-      (forall h lt. dec h lt ==> enforced_locally pi h lt) /\
-      (forall res. inside_respects_pi (k res) pi)
-
-
-let run_m
-  (pi:monitorable_prop)
-  (m : iio (Universe.raise_t 'b))
-  dec
-  k
-  p
-  (h:trace)
-  (_:squash (inside_respects_pi (Decorated dec m k) pi))
-  (_:squash (dm_iio_theta (Decorated dec m k) p h)) :
-//  (_:squash ) :
-  IIO 
-    (iio _ * _ * trace)
-    (requires (fun h' -> h == h'))
-    (ensures (fun h (z', p', h') lt ->
-      h' == apply_changes h lt /\
-      dm_iio_theta z' p' h' /\
-      enforced_locally pi h lt /\ 
-      inside_respects_pi z' pi)) =
-  assert (forall h lt. dec h lt ==> enforced_locally pi h lt);
-  super_lemma pi m dec k p h () ();
-  let theMHistPost : trace -> _ -> trace -> Type0 = (fun h r lt -> enforced_locally pi h lt) in
-  let theMHist : hist _ = to_hist (fun h' -> h == h') theMHistPost in
-  let theM : unit -> IIOwp _ theMHist = (fun () -> IIOwp?.reflect m) in
-  let resM = theM () in 
-  Classical.forall_intro (lemma_suffixOf_append h);
-  let ltM = IIO.CompileTo.ILang.extract_local_trace h pi in
-
-  let z' = k (Universe.downgrade_val resM) in
-  assert (dm_iio_theta m (fun lt r -> theMHistPost h r lt) h);
-  assert (dm_iio_theta m
-        (fun lt r ->
-          dm_iio_theta (k (Universe.downgrade_val r))
-            (hist_post_shift p lt)
-            (apply_changes h lt)) h);
-
- // assert (theMHist `hist_ord` dm_iio_theta m);
-  //assert (p lt res);
-  let p' = hist_post_shift p ltM in
-  let h' = apply_changes h ltM in
-  (** urgent - it is urgent, because I am not confident it can be proved **)
-  assert (dm_iio_theta z' p' h') by (tadmit ());
-  (z', p', h')
-
-(** not urgent assume **)
-assume val dynamic_cmd :
-  (cmd : io_cmds) ->
-  (d1 : checkable2 (io_pre cmd)) ->
-  (arg : io_sig.args cmd) ->
-  IIOwp (io_resm cmd)
-    (fun p h ->
-      (forall (r:(io_sig.res cmd arg)) lt.
-        (match r with
-         | Inr Contract_failure -> ~(d1.check2 arg h) /\ lt == []
-         | _ -> d1.check2 arg h /\ lt == [convert_call_to_event cmd arg r]) ==> p lt r))
-
-(** this is working but needs more help to verify **)
-let rec _instrument
-  (tree : iio (resexn 'a))
-  (p    : hist_post (resexn 'a))
-  (h    : trace)
-  (d1   : squash (dm_iio_theta tree p h))
-  (pi   : monitorable_prop)
-  (d2   : squash (inside_respects_pi tree pi))
-  (c_pi:squash (forall h cmd arg. pi cmd arg h ==> io_pre cmd arg h)) :
-  IIOwp (resexn 'a) (fun p h' -> h == h' /\ (forall lt r. enforced_locally pi h lt ==> p lt r)) =
-  match tree with
-  | Return r -> r
-  | Call GetTrace argz fnc -> Inr Contract_failure
-  | PartialCall pre fnc -> Inr Contract_failure
-  | Decorated d #b m k ->
-    admit ();
-    let (z', p', h') = run_m pi m d k p h d1 d2 in
-    _instrument z' p' h' () pi () c_pi
-  | Call cmd argz fnc -> begin
-    admit ();
-    let d : checkable2 (io_pre cmd) = (
-      implies_is_checkable2 (io_sig.args cmd) trace (pi cmd) (io_pre cmd) c_pi) in
-    (** Check if the runtime check failed, and if yes, return the error **)
-    let rez = dynamic_cmd cmd d argz in
-    let z' : iio (resexn 'a) = fnc rez in
-
-    let p' : hist_post (resexn 'a) = hist_post_shift p [convert_call_to_event cmd argz rez] in
-    let h' = apply_changes h [convert_call_to_event cmd argz rez] in
-    let proof1 : squash (dm_iio_theta z' p' h') = () in
-    let proof2 : squash (inside_respects_pi z' pi) = () in
-    _instrument z' p' h' proof1 pi proof2 c_pi
-  end
-
-let rec lemma_super_lemma (m:iio (resexn 'a)) pi :
-  Lemma (MIO.basic_free m ==> inside_respects_pi m pi) =
-  match m with
-  | Return _ -> ()
-  | Decorated _ _ _ -> ()
-  | PartialCall _ _ -> ()
-  | Call GetTrace _ _ -> ()
-  | Call cmd arg k ->
-    introduce forall res. MIO.basic_free (k res) ==> inside_respects_pi (k res) pi with begin
-      lemma_super_lemma (k res) pi
-    end
-
 instance instrumentable_unverified_arrow t1 t2 pi {| d1:compilable t1 pi |} {| d2:backtranslateable t2 pi |} : instrumentable t1 t2 pi = {
   mlang_inst_in = mlang_unverified_arrow d1.mlang_comp_out d2.mlang_btrans_in;
 
@@ -300,12 +132,9 @@ instance instrumentable_unverified_arrow t1 t2 pi {| d1:compilable t1 pi |} {| d
 
   c_pi = d2.cc_pi;
 
-  instrument = (fun f x -> 
-    let tree : MIO.dm_mio _ trivial_hist = reify (f (compile x)) in
-    let p = fun _ _ -> True in
-    let h = get_trace () in
-    lemma_super_lemma tree pi;
-    let r  : resexn d2.btrans_in = _instrument #d2.btrans_in tree p h () pi () d2.cc_pi in 
+  instrument = (fun (f:unverified_arrow d1.comp_out d2.btrans_in) (x:t1) -> 
+    let dm = reify (f (compile x)) in
+    let r  : resexn d2.btrans_in = instrument_mio dm () pi d2.cc_pi in 
     backtranslate #_ #pi #(backtranslateable_resexn pi t2 #d2) r 
   )
 }
