io/MLang.InstrumentTo.ILang.fst
@@ -1,0 +1,196 @@
+module MLang.InstrumentTo.ILang
+
+open FStar.List.Tot
+open FStar.Tactics
+
+open Common
+open TC.Checkable
+open TC.Monitorable.Hist
+open IO.Sig
+open IIO
+open ILang
+
+let basic_free = MIO.basic_free
+let mio = MIO.mio
+
+let super_lemma 
+  (pi:monitorable_prop)
+  (m : iio (Universe.raise_t 'b))
+  d
+  k
+  p
+  (h:trace)
+  (_:squash (dm_iio_theta (Decorated d m k) p h))
+  (_:squash (forall h lt. d h lt ==> enforced_locally pi h lt)) :
+  Lemma (
+   dm_iio_theta m (fun lt r -> enforced_locally pi h lt) h /\
+   dm_iio_theta m
+      (fun lt r ->
+        dm_iio_theta (k (Universe.downgrade_val r))
+          (hist_post_shift p lt)
+          (apply_changes h lt)) h) = admit ()
+ (** 
+  calc (==>) {
+      dm_iio_theta (Decorated d m k) p h;
+      ==> { _ by (
+            binder_retype (nth_binder (-1));
+            norm [delta_only [`%dm_iio_theta;`%DMFree.theta]; zeta];
+            trefl ();
+            norm [delta_only [`%dm_iio_theta]];
+            assumption ()) }
+      hist_bind
+             (fun p h -> dm_iio_theta m (fun lt r -> d h lt /\ p lt r) h)
+             (fun r -> dm_iio_theta (k (Universe.downgrade_val r))) p h;
+      ==> {}
+      hist_bind
+             (fun p h -> dm_iio_theta m (fun lt r -> enforced_locally pi h lt /\ p lt r) h)
+             (fun r -> dm_iio_theta (k (Universe.downgrade_val r))) p h;
+      ==> { _ by (binder_retype (nth_binder (-1));
+                  norm [delta_only [`%hist_bind;`%hist_post_bind]]; trefl (); assumption ()) }
+      dm_iio_theta m
+        (fun lt r ->
+          enforced_locally pi h lt /\
+          dm_iio_theta (k (Universe.downgrade_val r))
+            (hist_post_shift p lt)
+            (List.Tot.Base.rev lt @ h)) h;
+      ==> {}
+      dm_iio_theta m
+        (fun lt r ->
+          dm_iio_theta (k (Universe.downgrade_val r))
+            (hist_post_shift p lt)
+            (List.Tot.Base.rev lt @ h)) h;
+    }
+
+**) 
+
+let lemma_smt_pat (pi:monitorable_prop) (h lt1 lt2:trace) :
+  Lemma (requires (
+    enforced_locally pi h lt1 /\
+    enforced_locally pi (apply_changes h lt1) lt2))
+    (ensures (
+    enforced_locally pi h (lt1 @ lt2))) [SMTPat (enforced_locally pi h (lt1@lt2))] = (** not urgent **) admit ()
+
+let rec inside_respects_pi
+  (tree : iio (resexn 'a))
+  (pi : monitorable_prop) : Type0 =
+  match tree with
+  | Return _ -> True
+  | PartialCall pre k ->
+      pre ==> (inside_respects_pi (k ()) pi)
+  | Call cmd arg k ->
+      forall res. inside_respects_pi (k res) pi
+  | Decorated dec m k ->
+      (forall h lt. dec h lt ==> enforced_locally pi h lt) /\
+      (forall res. inside_respects_pi (k res) pi)
+
+
+let run_m
+  (pi:monitorable_prop)
+  (m : iio (Universe.raise_t 'b))
+  dec
+  k
+  p
+  (h:trace)
+  (_:squash (inside_respects_pi (Decorated dec m k) pi))
+  (_:squash (dm_iio_theta (Decorated dec m k) p h)) :
+//  (_:squash ) :
+  IIO 
+    (iio _ * _ * trace)
+    (requires (fun h' -> h == h'))
+    (ensures (fun h (z', p', h') lt ->
+      h' == apply_changes h lt /\
+      dm_iio_theta z' p' h' /\
+      enforced_locally pi h lt /\ 
+      inside_respects_pi z' pi)) =
+  assert (forall h lt. dec h lt ==> enforced_locally pi h lt);
+  super_lemma pi m dec k p h () ();
+  let theMHistPost : trace -> _ -> trace -> Type0 = (fun h r lt -> enforced_locally pi h lt) in
+  let theMHist : hist _ = to_hist (fun h' -> h == h') theMHistPost in
+  let theM : unit -> IIOwp _ theMHist = (fun () -> IIOwp?.reflect m) in
+  let resM = theM () in 
+  Classical.forall_intro (lemma_suffixOf_append h);
+  let ltM = IIO.CompileTo.ILang.extract_local_trace h pi in
+
+  let z' = k (Universe.downgrade_val resM) in
+  assert (dm_iio_theta m (fun lt r -> theMHistPost h r lt) h);
+  assert (dm_iio_theta m
+        (fun lt r ->
+          dm_iio_theta (k (Universe.downgrade_val r))
+            (hist_post_shift p lt)
+            (apply_changes h lt)) h);
+
+ // assert (theMHist `hist_ord` dm_iio_theta m);
+  //assert (p lt res);
+  let p' = hist_post_shift p ltM in
+  let h' = apply_changes h ltM in
+  (** urgent - it is urgent, because I am not confident it can be proved **)
+  assert (dm_iio_theta z' p' h') by (tadmit ());
+  (z', p', h')
+
+(** not urgent assume **)
+assume val dynamic_cmd :
+  (cmd : io_cmds) ->
+  (d1 : checkable2 (io_pre cmd)) ->
+  (arg : io_sig.args cmd) ->
+  IIOwp (io_resm cmd)
+    (fun p h ->
+      (forall (r:(io_sig.res cmd arg)) lt.
+        (match r with
+         | Inr Contract_failure -> ~(d1.check2 arg h) /\ lt == []
+         | _ -> d1.check2 arg h /\ lt == [convert_call_to_event cmd arg r]) ==> p lt r))
+
+(** this is working but needs more help to verify **)
+let rec _instrument
+  (tree : iio (resexn 'a))
+  (p    : hist_post (resexn 'a))
+  (h    : trace)
+  (d1   : squash (dm_iio_theta tree p h))
+  (pi   : monitorable_prop)
+  (d2   : squash (inside_respects_pi tree pi))
+  (c_pi:squash (forall h cmd arg. pi cmd arg h ==> io_pre cmd arg h)) :
+  IIOwp (resexn 'a) (fun p h' -> h == h' /\ (forall lt r. enforced_locally pi h lt ==> p lt r)) =
+  match tree with
+  | Return r -> r
+  | Call GetTrace argz fnc -> Inr Contract_failure
+  | PartialCall pre fnc -> Inr Contract_failure
+  | Decorated d #b m k ->
+    admit ();
+    let (z', p', h') = run_m pi m d k p h d1 d2 in
+    _instrument z' p' h' () pi () c_pi
+  | Call cmd argz fnc -> begin
+    admit ();
+    let d : checkable2 (io_pre cmd) = (
+      implies_is_checkable2 (io_sig.args cmd) trace (pi cmd) (io_pre cmd) c_pi) in
+    (** Check if the runtime check failed, and if yes, return the error **)
+    let rez = dynamic_cmd cmd d argz in
+    let z' : iio (resexn 'a) = fnc rez in
+
+    let p' : hist_post (resexn 'a) = hist_post_shift p [convert_call_to_event cmd argz rez] in
+    let h' = apply_changes h [convert_call_to_event cmd argz rez] in
+    let proof1 : squash (dm_iio_theta z' p' h') = () in
+    let proof2 : squash (inside_respects_pi z' pi) = () in
+    _instrument z' p' h' proof1 pi proof2 c_pi
+  end
+
+let rec lemma_super_lemma (m:iio (resexn 'a)) pi :
+  Lemma (basic_free m ==> inside_respects_pi m pi) =
+  match m with
+  | Return _ -> ()
+  | Decorated _ _ _ -> ()
+  | PartialCall _ _ -> ()
+  | Call GetTrace _ _ -> ()
+  | Call cmd arg k ->
+    introduce forall res. basic_free (k res) ==> inside_respects_pi (k res) pi with begin
+      lemma_super_lemma (k res) pi
+    end
+
+let instrument_mio
+  (tree:mio (resexn 'a))
+  (_:squash (trivial_hist `hist_ord` dm_iio_theta tree))
+  (pi   : monitorable_prop)
+  (c_pi:squash (forall h cmd arg. pi cmd arg h ==> io_pre cmd arg h)) :
+  IIOpi (resexn 'a) pi = 
+  let p = fun _ _ -> True in
+  let h = get_trace () in
+  lemma_super_lemma tree pi;
+  _instrument tree p h () pi () c_pi
